sort -> type

coq/Alg.v
@@ -1,6 +1,6 @@
 (** * The Message Algebra *)
 
-Require Import Nat DecBool Monad Proc.
+Require Import FunInd Nat Bool DecBool Monad Proc.
 (** printing <- #←# *)
 
 Notation var := nat (only parsing).
@@ -67,6 +67,31 @@ Proof.
     decide equality.
 Defined.
 Hint Resolve alg_dec : core.
+
+Definition alg_eqb x y: bool :=
+  if alg_dec x y then
+    true
+  else
+    false.
+
+Lemma alg_eq_correct:
+  forall x y,
+    alg_eqb x y = true <-> x = y.
+Proof.
+  intros.
+  unfold alg_eqb.
+  destruct (alg_dec x y); subst; intuition.
+  inversion H.
+Qed.
+
+Lemma alg_eq_complete:
+  forall x y,
+    alg_eqb x y = false <-> x <> y.
+Proof.
+  intros.
+  unfold alg_eqb.
+  destruct (alg_dec x y); subst; intuition.
+Qed.
 
 (** Event *)
 
@@ -151,9 +176,9 @@ Proof.
     rewrite inv_inv; auto.
 Qed.
 
-(** ** Sort of an Algebra Term *)
+(** ** Type of an Algebra Term *)
 
-Definition sort_of (x: alg): sort :=
+Definition type_of (x: alg): type :=
   match x with
   | Tx v => Text
   | Dt v => Data
@@ -167,12 +192,12 @@ Definition sort_of (x: alg): sort :=
 
 (** ** Is a Term Well Formed?
 
-    When a term is well formed, variables must have a consistent sort.
+    When a term is well formed, variables must have a consistent type.
     An example of a term that is not well formed is
 <<
     Pr (Tx 0) (Nm 0)
 >>
-    The sort of variable 0 can't be both [Text] and [Name].
+    The type of variable 0 can't be both [Text] and [Name].
  *)
 
 (** Lookup [v] in association list [e]. *)
@@ -190,13 +215,13 @@ Fixpoint lookup {A} (v: var) (e: list (var * A)): option A :=
 (** Extend the decls if the extension is consistent with previous
     declarations. *)
 
-Definition extend decls (v: var) (s: sort): option (list decl) :=
+Definition extend decls (v: var) (s: type): option (list decl) :=
   match lookup v decls with
   | None => Some ((v, s) :: decls)
   | Some s' =>
-    if sort_dec s' s then
+    if type_dec s' s then
       Some decls
-    else                        (* Sort clash! *)
+    else                        (* Type clash! *)
       None
   end.
 
@@ -254,63 +279,63 @@ Definition well_formed_event decls (x: evt): option (list decl) :=
     well_formed ds y
   end.
 
-(** ** Is a Term Well Sorted?
+(** ** Is a Term Well Typed?
 
     Like well formed except it does not extend its declarations. *)
 
-Definition well_sorted_var decls (v: var) (s: sort): bool :=
+Definition well_typed_var decls (v: var) (s: type): bool :=
   match lookup v decls with
   | None => false
-  | Some s' => ifdec (sort_dec s' s) true false
+  | Some s' => ifdec (type_dec s' s) true false
   end.
 
-(** Is skey well sorted? *)
+(** Is skey well typed? *)
 
-Definition well_sorted_skey decls (k: skey): bool :=
+Definition well_typed_skey decls (k: skey): bool :=
   match k with
-  | Sv v => well_sorted_var decls v Skey
-  | Lt v v' => well_sorted_var decls v Name &&
-               well_sorted_var decls v' Name
+  | Sv v => well_typed_var decls v Skey
+  | Lt v v' => well_typed_var decls v Name &&
+               well_typed_var decls v' Name
   end.
 
-(** Is akey well sorted? *)
+(** Is akey well typed? *)
 
-Definition well_sorted_akey decls (k: akey): bool :=
+Definition well_typed_akey decls (k: akey): bool :=
   match k with
-  | Av v => well_sorted_var decls v Akey
-  | Pb v =>  well_sorted_var decls v Name
-  | Pb2 c v =>  well_sorted_var decls v Name
+  | Av v => well_typed_var decls v Akey
+  | Pb v =>  well_typed_var decls v Name
+  | Pb2 c v =>  well_typed_var decls v Name
   end.
 
-(** Is algebra term well sorted?  For term [x], [well_sorted decl x]
-    is true when [x] is true when it is well sorted with respect to
+(** Is algebra term well typed?  For term [x], [well_typed decl x]
+    is true when [x] is true when it is well typed with respect to
     the declarations [decls].  Note that channels are considered not
-    well sorted in this function. *)
+    well typed in this function. *)
 
-Fixpoint well_sorted decls (x: alg): bool :=
+Fixpoint well_typed decls (x: alg): bool :=
   match x with
-  | Tx v => well_sorted_var decls v Text
-  | Dt v => well_sorted_var decls v Data
-  | Nm v => well_sorted_var decls v Name
-  | Sk k => well_sorted_skey decls k
-  | Ak k => well_sorted_akey decls k
-  | Ik k => well_sorted_akey decls k
+  | Tx v => well_typed_var decls v Text
+  | Dt v => well_typed_var decls v Data
+  | Nm v => well_typed_var decls v Name
+  | Sk k => well_typed_skey decls k
+  | Ak k => well_typed_akey decls k
+  | Ik k => well_typed_akey decls k
   | Ch v => false               (* Channels are forbidden *)
-  | Mg v => well_sorted_var decls v Mesg
+  | Mg v => well_typed_var decls v Mesg
   | Tg z => true
-  | Pr y z => well_sorted decls y &&
-              well_sorted decls z
-  | En y z => well_sorted decls y &&
-              well_sorted decls z
-  | Hs y => well_sorted decls y
+  | Pr y z => well_typed decls y &&
+              well_typed decls z
+  | En y z => well_typed decls y &&
+              well_typed decls z
+  | Hs y => well_typed decls y
   end.
 
-(** Is algebra term or channel well sorted? *)
+(** Is algebra term or channel well typed? *)
 
-Definition well_sorted_with_chan decls (x: alg): bool :=
+Definition well_typed_with_chan decls (x: alg): bool :=
   match x with
-  | Ch v => well_sorted_var decls v Chan
-  | _ => well_sorted decls x
+  | Ch v => well_typed_var decls v Chan
+  | _ => well_typed decls x
   end.
 
 (** ** Measure of a term *)
@@ -334,15 +359,92 @@ Qed.
 
 (** Carried by *)
 
+(** Carried by *)
+
 Fixpoint cb (x y: alg): bool :=
-  if alg_dec x y then
-    true
-  else
-    match y with
-    | Pr a b => cb x a || cb x b
-    | En a _ => cb x a
-    | _ => false
-    end.
+  alg_eqb x y ||
+          match y with
+          | Pr a b => cb x a || cb x b
+          | En a _ => cb x a
+          | _ => false
+          end.
+
+Functional Scheme cb_ind :=
+  Induction for cb Sort Prop.
+
+Lemma cb_refl:
+  forall x,
+    cb x x = true.
+Proof.
+  intros.
+  cut (alg_eqb x x = true); intros.
+  - destruct x; simpl; rewrite H; auto.
+  - apply alg_eq_correct; auto.
+Qed.
+
+Inductive carried_by: alg -> alg -> Prop :=
+| Carried_by_refl:
+    forall x, carried_by x x
+| Carried_by_frst:
+    forall x y z,
+      carried_by z x ->
+      carried_by z (Pr x y)
+| Carried_by_scnd:
+    forall x y z,
+      carried_by z y ->
+      carried_by z (Pr x y)
+| Carried_by_decr:
+    forall x y z,
+      carried_by z x ->
+      carried_by z (En x y).
+Hint Constructors carried_by : core.
+
+Lemma carried_by_trans:
+  forall x y z,
+    carried_by x y ->
+    carried_by y z ->
+    carried_by x z.
+Proof.
+  intros.
+  induction H0; simpl; auto.
+Qed.
+
+Lemma carried_by_reflect:
+  forall x y,
+    cb x y = true <-> carried_by x y.
+Proof.
+  split; intros.
+  - functional induction (cb x y);
+      try inversion H; auto; apply orb_true_iff in H;
+        destruct H; try inversion H;
+          try (apply alg_eq_correct in H; subst; auto).
+    + apply orb_true_iff in H.
+      destruct H.
+      * apply IHb in H; auto.
+      * apply IHb0 in H; auto.
+    + apply IHb in H; auto.
+  - induction H.
+    + apply cb_refl.
+    + destruct (alg_dec z (Pr x y)) as [G|G]; subst.
+      * apply cb_refl.
+      * rewrite <- alg_eq_complete in G.
+        destruct x; unfold cb; rewrite G; fold cb;
+          simpl in IHcarried_by; apply orb_true_iff in IHcarried_by;
+            destruct IHcarried_by; try inversion IHcarried_by;
+              try rewrite H0; simpl; auto; repeat rewrite orb_true_iff; auto.
+    + destruct (alg_dec z (Pr x y)) as [G|G]; subst.
+      * apply cb_refl.
+      * rewrite <- alg_eq_complete in G.
+        destruct x; unfold cb; rewrite G; fold cb; rewrite IHcarried_by;
+          repeat rewrite orb_true_iff; auto.
+    + destruct (alg_dec z (En x y)) as [G|G]; subst.
+      * apply cb_refl.
+      * rewrite <- alg_eq_complete in G.
+        destruct x; unfold cb; rewrite G; fold cb;
+          simpl in IHcarried_by; apply orb_true_iff in IHcarried_by;
+            destruct IHcarried_by; try inversion IHcarried_by;
+              try rewrite H0; simpl; auto; repeat rewrite orb_true_iff; auto.
+Qed.
 
 (** Does [x] originate in [tr]? *)
 
